lean/PartialOrder.lean
@@ -1,0 +1,32 @@
+/-
+  Defines PartialOrder and PartialOrderSq, along with notation
+  for the latter.
+-/
+
+-- The square less-equal relation: `x ⊑ y`.
+class SqLE (α : Type u) where
+  le : α → α → Prop
+
+-- The square less-equal relation: `x ⊏ y`.
+class SqLT (α : Type u) where
+  lt : α → α → Prop
+
+infix:50 " ⊑ " => SqLE.le
+infix:50 " ⊏ " => SqLT.lt
+
+class PartialOrder (T: Type) extends LE T, LT T where
+  refl (t: T): t ≤ t
+  antisymm (a b: T): a ≤ b  →  b ≤ a  →  a = b
+  trans (a b c: T): a ≤ b  →  b ≤ c  →  a ≤ c
+  
+  lt (a b: T) := a ≤ b  ∧  ¬ a = b
+  ltIffLeNotEq (a b: T): a < b  ↔  a ≤ b ∧ ¬ a = b
+
+-- Can I combine PartialOrder with PartialOrderSq into one definition?
+class PartialOrderSq (T: Type) extends SqLE T, SqLT T where
+  refl (t: T): t ⊑ t
+  antisymm (a b: T): a ⊑ b  →  b ⊑ a  →  a = b
+  trans (a b c: T): a ⊑ b  →  b ⊑ c  →  a ⊑ c
+  
+  lt (a b: T) := a ⊑ b  ∧  ¬ a = b
+  ltIffLeNotEq (a b: T): a ⊏ b  ↔  a ⊑ b ∧ ¬ a = b
