lean/lakefile.lean
@@ -1,0 +1,8 @@
+import Lake
+open Lake DSL
+
+package Bst {
+  isLeanOnly := true
+}
+
+lean_lib PartialOrder {}
